---
title: "Worksheet 3"
author: Wenje Tu
date: "Spring Semester 2022"
output: pdf_document
# bibliography: biblio.bib
# nocite: '@*'
subtitle: Foundations of Bayesian Methodology
papersize: a4
fontsize: 10pt
---

```{r setup, include=FALSE}
knitr::opts_chunk$set(echo = TRUE)
```

### Exercise 3 (Conjugate Bayes: analytical derivation)

Assumptions: 
$$
\begin{aligned}
y_1,\cdots,y_n\mid m  & \overset{i.i.d}{\sim} \mathcal{N}(m,\kappa^{-1}) \\
m & \: \sim \:\mathcal{N}(\mu,\lambda^{-1})
\end{aligned}
$$

**3 (a)**

Prior distribution: 
$$
f(m)=\sqrt{\frac{\lambda}{2\pi}}\exp\left(-\frac{\lambda}{2}(m-\mu)^2 \right)
$$

The prior predictive distribution of one future observation $y$ assuming that no observations have been collected yet:
$$
\begin{aligned}
f(y)
&=\int_{-\infty}^{\infty}f(y, m)\text{d}m
\quad\color{red}{\text{marginalize over its prior distribution}} \\
&=\int_{-\infty}^{\infty}f(y\mid m)f(m)\text{d}m \\
&=\int_{-\infty}^{\infty}\sqrt{\frac{\kappa}{2\pi}}\exp\left(-\frac{\kappa}{2}(y-m)^2 \right)
\sqrt{\frac{\lambda}{2\pi}}\exp\left(-\frac{\lambda}{2}(m-\mu)^2 \right)\text{d}m \\
&=\frac{\sqrt{\kappa\lambda}}{2\pi}\int_{-\infty}^{\infty}
\exp\left(-\frac{1}{2}\left(\kappa(y^2-2ym+m^2)+\lambda(m^2-2m\mu+\mu^2) \right) \right)\text{d}m \\
&=\frac{\sqrt{\kappa\lambda}}{2\pi}\int_{-\infty}^{\infty}
\exp\left(-\frac{1}{2}\left((\kappa+\lambda)\left(m-\frac{\kappa y+\lambda\mu}{\kappa+\lambda} \right)^2
-\frac{(\kappa y+\lambda\mu)^2}{\kappa+\lambda}+\kappa y^2+\lambda \mu^2
\right) \right)\text{d}m \\
&=\frac{\sqrt{\kappa\lambda}}{2\pi}\int_{-\infty}^{\infty}
\exp\left(-\frac{1}{2}\left((\kappa+\lambda)\left(m-\frac{\kappa y+\lambda\mu}{\kappa+\lambda} \right)^2
+\frac{\kappa\lambda(y-\mu)^2}{\kappa+\lambda}
\right) \right)\text{d}m \\
&=\frac{\sqrt{\kappa\lambda}}{2\pi}\exp\left(-\frac{\kappa\lambda(y-\mu)^2}{2(\kappa+\lambda)}\right)
\int_{-\infty}^{\infty}
\exp\left(-\frac{\kappa+\lambda}{2}\left(m-\frac{\kappa y+\lambda\mu}{\kappa+\lambda} \right)^2
\right)\text{d}m \\
&=\frac{\sqrt{\kappa\lambda}}{2\pi}\sqrt{\frac{2\pi}{\kappa+\lambda}}
\exp\left(-\frac{\kappa\lambda(y-\mu)^2}{2(\kappa+\lambda)}\right)
\underbrace{
\int_{-\infty}^{\infty}\sqrt{\frac{\kappa+\lambda}{2\pi}}
\exp\left(-\frac{\kappa+\lambda}{2}\left(m-\frac{\kappa y+\lambda\mu}{\kappa+\lambda} \right)^2
\right)\text{d}m}_{=1} \\
&=\frac{\sqrt{\kappa\lambda}}{2\pi}\sqrt{\frac{2\pi}{\kappa+\lambda}}
\exp\left(-\frac{\kappa\lambda(y-\mu)^2}{2(\kappa+\lambda)}\right) \\
&=\sqrt{\frac{1}{2\pi\left(\frac{1}{\lambda}+\frac{1}{\kappa} \right)}}
\exp\left(-\frac{(y-\mu)^2}{2\left(\frac{1}{\lambda}+\frac{1}{\kappa} \right)}\right)
\end{aligned}
$$

The prior predictive distribution of one future observation $y$ is
$$
\mathcal{N}(\mu, \lambda^{-1}+\kappa^{-1})
$$

**3 (b)**

In worksheet 2, we have already derived the posterior distribution:
$$
m\mid y_1,\cdots,y_n\sim \mathcal{N}
\left(\frac{\kappa n\bar{y}+\lambda\mu}{n\kappa+\lambda}, \frac{1}{n\kappa+\lambda}\right)
$$

Denote:
$$
\begin{aligned}
  \mu_\text{post} &= \frac{\kappa n\bar{y}+\lambda\mu}{n\kappa+\lambda} \\
  \lambda_\text{post} &= n\kappa+\lambda
\end{aligned}
$$

$$
\begin{aligned}
f(m\mid y_1,\cdots, y_n)
&=\sqrt{\frac{n\kappa+\lambda}{2\pi}}\exp\left(-\frac{n\kappa+\lambda}{2}\left(m-\frac{\kappa n\bar{y}+\lambda\mu}{n\kappa+\lambda} \right)^2  \right) \\
&=\sqrt{\frac{\lambda_\text{post}}{2\pi}}\exp\left(-\frac{\lambda_\text{post}}{2}\left(m-\mu_\text{post} \right)^2  \right)
\end{aligned}
$$


The posterior predictive distribution of one future observation $y_{n+1}$ given that $y_1,\cdots,y_n$ have been observed:
$$
\begin{aligned}
f(y_{n+1}\mid y_1,\cdots,y_n)
&=\int_{-\infty}^{\infty}f(y_{n+1},m\mid y_1,\cdots,y_n)\text{d}m
\quad\color{red}{\text{marginalize over its posterior distribution}} \\
&=\int_{-\infty}^{\infty}f(y_{n+1}\mid m, y_1,\cdots,y_n)f(m\mid y_1,\cdots,y_n)\text{d}m \\
&=\int_{-\infty}^{\infty}f(y_{n+1}\mid m)f(m\mid y_1,\cdots,y_n)\text{d}m \\
&=\int_{-\infty}^{\infty}\sqrt{\frac{\kappa}{2\pi}}\exp\left(-\frac{\kappa}{2}(y_{n+1}-m)^2 \right)
\underbrace{\sqrt{\frac{\lambda_\text{post}}{2\pi}}\exp\left(-\frac{\lambda_\text{post}}{2}\left(m-\mu_\text{post} \right)^2  \right)}_{\text{posterior distribution}}\text{dm} \\
&\:\:\vdots\quad\text{repeat the same steps as for the prior predictive distribution} \\
&=\sqrt{\frac{1}{2\pi\left(\frac{1}{\lambda_\text{post}}+\frac{1}{\kappa} \right)}}
\exp\left(-\frac{(y-\mu_\text{post})^2}{2\left(\frac{1}{\lambda_\text{post}}+\frac{1}{\kappa} \right)}\right)
\end{aligned}
$$

$$
y_{n+1}\mid y_1,\cdots,y_n\sim\mathcal{N}(\mu_\text{post}, \lambda_\text{post}^{-1}+\kappa^{-1})
$$
